Refactor pattern_interpretation into eval

matching-logic/src/Semantics.v
@@ -21,7 +21,7 @@ From MatchingLogic Require Import
 Import MatchingLogic.Syntax.Notations.
 (** ** Matching Logic Semantics *)
 Section semantics.
-  
+
   Context {signature : Signature}.
 
   (* Model of AML ref. snapshot: Definition 2 *)
@@ -254,7 +254,7 @@ Section semantics.
     Let OS := PropsetOrderedSet (@Domain m).
     Let  L := PowersetLattice (@Domain m).
 
-    Program Fixpoint pattern_interpretation
+    Program Fixpoint eval
             (evar_val : evar -> Domain m) (svar_val : svar -> propset (Domain m))
             (p : Pattern) {measure (size p)} :=
       match p with
@@ -263,21 +263,21 @@ Section semantics.
       | patt_bound_evar x => ∅
       | patt_bound_svar X => ∅
       | patt_sym s => (@sym_interp m) s
-      | patt_app ls rs => app_ext (pattern_interpretation evar_val svar_val ls)
-                                  (pattern_interpretation evar_val svar_val rs)
+      | patt_app ls rs => app_ext (eval evar_val svar_val ls)
+                                  (eval evar_val svar_val rs)
       | patt_bott => ∅
-      | patt_imp ls rs => (difference ⊤ (pattern_interpretation evar_val svar_val ls)) ∪
-                                          (pattern_interpretation evar_val svar_val rs)
+      | patt_imp ls rs => (difference ⊤ (eval evar_val svar_val ls)) ∪
+                                          (eval evar_val svar_val rs)
       | patt_exists p' =>
         let x := fresh_evar p' in
         propset_fa_union
-          (fun e => pattern_interpretation (update_evar_val x e evar_val)
+          (fun e => eval (update_evar_val x e evar_val)
                                            svar_val
                                            (evar_open 0 x p'))
       | patt_mu p' =>
         let X := fresh_svar p' in
         @LeastFixpointOf _ OS L
-                         (fun S => pattern_interpretation evar_val
+                         (fun S => eval evar_val
                                                           (update_svar_val X S svar_val)
                                                           (svar_open 0 X p'))
       end.
@@ -291,58 +291,58 @@ Section semantics.
 
 
     Definition Fassoc ρₑ ρₛ ϕ X :=
-      λ S, pattern_interpretation ρₑ (update_svar_val X S ρₛ) ϕ.
+      λ S, eval ρₑ (update_svar_val X S ρₛ) ϕ.
     
     (* TODO: Need to be able to simplify Program Fixpoint definitions *)
 
-    Lemma pattern_interpretation_free_evar_simpl
+    Lemma eval_free_evar_simpl
           (evar_val : evar -> Domain m) (svar_val : svar -> propset (Domain m))
           (x : evar) :
-      pattern_interpretation evar_val svar_val (patt_free_evar x) = {[ evar_val x ]}.
+      eval evar_val svar_val (patt_free_evar x) = {[ evar_val x ]}.
     Proof.
       auto.
     Qed.
 
-    Lemma pattern_interpretation_free_svar_simpl
+    Lemma eval_free_svar_simpl
           (evar_val : evar -> Domain m) (svar_val : svar -> propset (Domain m))
           (X : svar) :
-      pattern_interpretation evar_val svar_val (patt_free_svar X) = svar_val X.
+      eval evar_val svar_val (patt_free_svar X) = svar_val X.
     Proof.
       auto.
     Qed.
 
-    Lemma pattern_interpretation_bound_evar_simpl
+    Lemma eval_bound_evar_simpl
           (evar_val : evar -> Domain m) (svar_val : svar -> propset (Domain m))
           (x : db_index) :
-      pattern_interpretation evar_val svar_val (patt_bound_evar x) = ∅.
+      eval evar_val svar_val (patt_bound_evar x) = ∅.
     Proof.
       auto.
     Qed.
 
-    Lemma pattern_interpretation_bound_svar_simpl
+    Lemma eval_bound_svar_simpl
           (evar_val : evar -> Domain m) (svar_val : svar -> propset (Domain m))
           (X : db_index) :
-      pattern_interpretation evar_val svar_val (patt_bound_svar X) = ∅.
+      eval evar_val svar_val (patt_bound_svar X) = ∅.
     Proof.
       auto.
     Qed.
 
-    Lemma pattern_interpretation_sym_simpl
+    Lemma eval_sym_simpl
           (evar_val : @EVarVal m) (svar_val : @SVarVal m)
           (s : symbols) :
-      pattern_interpretation evar_val svar_val (patt_sym s) = @sym_interp m s.
+      eval evar_val svar_val (patt_sym s) = @sym_interp m s.
     Proof.
       auto.
     Qed.
 
-    Lemma pattern_interpretation_app_simpl
+    Lemma eval_app_simpl
           (evar_val : evar -> Domain m) (svar_val : svar -> propset (Domain m))
           (ls rs : Pattern) :
-      pattern_interpretation evar_val svar_val (patt_app ls rs) =
-      app_ext (pattern_interpretation evar_val svar_val ls)
-              (pattern_interpretation evar_val svar_val rs).
+      eval evar_val svar_val (patt_app ls rs) =
+      app_ext (eval evar_val svar_val ls)
+              (eval evar_val svar_val rs).
     Proof.
-      unfold pattern_interpretation, pattern_interpretation_func.
+      unfold eval, eval_func.
       rewrite fix_sub_eq.
       intros x f g Heq.
       destruct x. Tactics.program_simpl. unfold projT1, projT2.
@@ -352,21 +352,21 @@ Section semantics.
       { f_equal. }
     Qed.
 
-    Lemma pattern_interpretation_bott_simpl
+    Lemma eval_bott_simpl
           (evar_val : evar -> Domain m) (svar_val : svar -> propset (Domain m)) :
-      pattern_interpretation evar_val svar_val patt_bott = ∅.
+      eval evar_val svar_val patt_bott = ∅.
     Proof.
       auto.
     Qed.
 
-    Lemma pattern_interpretation_imp_simpl
+    Lemma eval_imp_simpl
           (evar_val : evar -> Domain m) (svar_val : svar -> propset (Domain m))
           (ls rs : Pattern) :
-      pattern_interpretation evar_val svar_val (patt_imp ls rs) =
-      (difference ⊤ (pattern_interpretation evar_val svar_val ls)) ∪
-                      (pattern_interpretation evar_val svar_val rs).
+      eval evar_val svar_val (patt_imp ls rs) =
+      (difference ⊤ (eval evar_val svar_val ls)) ∪
+                      (eval evar_val svar_val rs).
     Proof.
-      unfold pattern_interpretation, pattern_interpretation_func.
+      unfold eval, eval_func.
       rewrite fix_sub_eq.
       intros x f g Heq.
       destruct x. Tactics.program_simpl. unfold projT1, projT2.
@@ -376,17 +376,17 @@ Section semantics.
       { f_equal. }
     Qed.
 
-    Lemma pattern_interpretation_ex_simpl
+    Lemma eval_ex_simpl
           (evar_val : evar -> Domain m) (svar_val : svar -> propset (Domain m))
           (p : Pattern) :
-      pattern_interpretation evar_val svar_val (patt_exists p) =
+      eval evar_val svar_val (patt_exists p) =
       let x := fresh_evar p in
       propset_fa_union 
-        (fun e => pattern_interpretation (update_evar_val x e evar_val)
+        (fun e => eval (update_evar_val x e evar_val)
                                          svar_val
                                          (evar_open 0 x p)).
     Proof.
-      unfold pattern_interpretation, pattern_interpretation_func.
+      unfold eval, eval_func.
       rewrite fix_sub_eq.
       intros x f g Heq.
       destruct x. Tactics.program_simpl. unfold projT1, projT2.
@@ -396,17 +396,17 @@ Section semantics.
       { f_equal. }
     Qed.
 
-    Lemma pattern_interpretation_mu_simpl
+    Lemma eval_mu_simpl
           (evar_val : evar -> Domain m) (svar_val : svar -> propset (Domain m))
           (p : Pattern) :
-      pattern_interpretation evar_val svar_val (patt_mu p) =
+      eval evar_val svar_val (patt_mu p) =
       let X := fresh_svar p in
       @LeastFixpointOf _ OS L
-                       (fun S => pattern_interpretation evar_val
+                       (fun S => eval evar_val
                                                         (update_svar_val X S svar_val)
                                                         (svar_open 0 X p)).
     Proof.
-      unfold pattern_interpretation, pattern_interpretation_func.
+      unfold eval, eval_func.
       rewrite fix_sub_eq.
       intros x f g Heq.
       destruct x. Tactics.program_simpl. unfold projT1, projT2.
@@ -417,17 +417,17 @@ Section semantics.
     Qed.
 
     (* TODO extend with derived constructs using typeclasses *)
-    Definition pattern_interpretation_simpl :=
-      ( pattern_interpretation_free_evar_simpl,
-        pattern_interpretation_free_svar_simpl,
-        pattern_interpretation_bound_evar_simpl,
-        pattern_interpretation_bound_svar_simpl,
-        pattern_interpretation_sym_simpl,  
-        pattern_interpretation_app_simpl,
-        pattern_interpretation_bott_simpl,
-        pattern_interpretation_imp_simpl,
-        pattern_interpretation_ex_simpl,
-        pattern_interpretation_mu_simpl
+    Definition eval_simpl :=
+      ( eval_free_evar_simpl,
+        eval_free_svar_simpl,
+        eval_bound_evar_simpl,
+        eval_bound_svar_simpl,
+        eval_sym_simpl,  
+        eval_app_simpl,
+        eval_bott_simpl,
+        eval_imp_simpl,
+        eval_ex_simpl,
+        eval_mu_simpl
       ).
 
 
@@ -440,13 +440,13 @@ Section semantics.
 
   (* Model predicate. Useful mainly if the pattern is well-formed. *)
   Definition M_predicate (M : Model) (ϕ : Pattern) : Prop := forall ρₑ ρ,
-      @pattern_interpretation M ρₑ ρ ϕ = ⊤ \/ pattern_interpretation ρₑ ρ ϕ = ∅.
+      @eval M ρₑ ρ ϕ = ⊤ \/ eval ρₑ ρ ϕ = ∅.
 
   Lemma M_predicate_impl M ϕ₁ ϕ₂ : M_predicate M ϕ₁ -> M_predicate M ϕ₂ -> M_predicate M (patt_imp ϕ₁ ϕ₂).
   Proof.
     unfold M_predicate. intros Hp1 Hp2 ρₑ ρ.
     specialize (Hp1 ρₑ ρ). specialize (Hp2 ρₑ ρ).
-    rewrite -> pattern_interpretation_imp_simpl.
+    rewrite -> eval_imp_simpl.
     destruct Hp1, Hp2; rewrite -> H; rewrite -> H0.
     + left. set_solver by fail.
     + right. set_solver by fail.
@@ -459,7 +459,7 @@ Section semantics.
   Lemma M_predicate_bott M : M_predicate M patt_bott.
   Proof.
     unfold M_predicate. intros. right.
-    apply pattern_interpretation_bott_simpl.
+    apply eval_bott_simpl.
   Qed.
 
   Hint Resolve M_predicate_bott : core.
@@ -469,11 +469,11 @@ Section semantics.
     M_predicate M (evar_open 0 x ϕ) -> M_predicate M (patt_exists ϕ).
   Proof.
     simpl. unfold M_predicate. intros.
-    rewrite -> pattern_interpretation_ex_simpl.
+    rewrite -> eval_ex_simpl.
     simpl.
     pose proof (H' := classic
                         (exists e : Domain M,
-                            (pattern_interpretation
+                            (eval
                                (update_evar_val (evar_fresh (elements (free_evars ϕ))) e ρₑ)
                                ρ
                                (evar_open 0 (evar_fresh (elements (free_evars ϕ))) ϕ))
@@ -511,8 +511,8 @@ Section semantics.
   
   Lemma predicate_not_empty_iff_full M ϕ ρₑ ρ :
     M_predicate M ϕ ->
-    @pattern_interpretation M ρₑ ρ ϕ <> ∅ <->
-    @pattern_interpretation M ρₑ ρ ϕ = ⊤.
+    @eval M ρₑ ρ ϕ <> ∅ <->
+    @eval M ρₑ ρ ϕ = ⊤.
   Proof.
     intros Hmp.
     split.
@@ -527,8 +527,8 @@ Section semantics.
 
   Lemma predicate_not_full_iff_empty M ϕ ρₑ ρ :
     M_predicate M ϕ ->
-    @pattern_interpretation M ρₑ ρ ϕ <> ⊤ <->
-    @pattern_interpretation M ρₑ ρ ϕ = ∅.
+    @eval M ρₑ ρ ϕ <> ⊤ <->
+    @eval M ρₑ ρ ϕ = ∅.
   Proof.
     intros Hmp.
     split.
@@ -541,31 +541,31 @@ Section semantics.
       assumption.
   Qed.
 
-  Lemma pattern_interpretation_impl_MP M ϕ₁ ϕ₂ ρₑ ρ :
-    @pattern_interpretation M ρₑ ρ (patt_imp ϕ₁ ϕ₂) = ⊤ ->
-    @pattern_interpretation M ρₑ ρ ϕ₁ = ⊤ ->
-    @pattern_interpretation M ρₑ ρ ϕ₂ = ⊤.
+  Lemma eval_impl_MP M ϕ₁ ϕ₂ ρₑ ρ :
+    @eval M ρₑ ρ (patt_imp ϕ₁ ϕ₂) = ⊤ ->
+    @eval M ρₑ ρ ϕ₁ = ⊤ ->
+    @eval M ρₑ ρ ϕ₂ = ⊤.
   Proof.
     unfold Full.
-    rewrite pattern_interpretation_imp_simpl.
+    rewrite eval_imp_simpl.
     intros H1 H2.
     rewrite -> H2 in H1.
     set_solver by auto.
   Qed.
 
-  Lemma pattern_interpretation_predicate_impl M ϕ₁ ϕ₂ ρₑ ρ :
+  Lemma eval_predicate_impl M ϕ₁ ϕ₂ ρₑ ρ :
     M_predicate M ϕ₁ ->
-    pattern_interpretation ρₑ ρ (patt_imp ϕ₁ ϕ₂) = ⊤
-    <-> (pattern_interpretation ρₑ ρ ϕ₁ = ⊤
-         -> @pattern_interpretation M ρₑ ρ ϕ₂ = ⊤).
+    eval ρₑ ρ (patt_imp ϕ₁ ϕ₂) = ⊤
+    <-> (eval ρₑ ρ ϕ₁ = ⊤
+         -> @eval M ρₑ ρ ϕ₂ = ⊤).
   Proof.
     intros Hpred.
     split.
     - intros H H1.
-      apply (pattern_interpretation_impl_MP H H1).
+      apply (eval_impl_MP H H1).
     - intros H.
-      rewrite -> pattern_interpretation_imp_simpl.
-      destruct (classic (pattern_interpretation ρₑ ρ ϕ₁ = ⊤)).
+      rewrite -> eval_imp_simpl.
+      destruct (classic (eval ρₑ ρ ϕ₁ = ⊤)).
       + specialize (H H0).
         rewrite -> H. rewrite -> H0.
         set_solver by fail.
@@ -575,15 +575,15 @@ Section semantics.
   Qed.
   
   (* ϕ is a well-formed body of ex *)
-  Lemma pattern_interpretation_exists_predicate_full M ϕ ρₑ ρ :
+  Lemma eval_exists_predicate_full M ϕ ρₑ ρ :
     let x := fresh_evar ϕ in
     M_predicate M (evar_open 0 x ϕ) ->
-    pattern_interpretation ρₑ ρ (patt_exists ϕ) = ⊤ <->
-    ∃ (m : Domain M), pattern_interpretation (update_evar_val x m ρₑ) ρ (evar_open 0 x ϕ) = ⊤.
+    eval ρₑ ρ (patt_exists ϕ) = ⊤ <->
+    ∃ (m : Domain M), eval (update_evar_val x m ρₑ) ρ (evar_open 0 x ϕ) = ⊤.
   Proof.
     intros x Hpred.
     pose proof (Hpredex := M_predicate_exists Hpred).
-    rewrite -[pattern_interpretation _ _ _ = ⊤]predicate_not_empty_iff_full. 2: auto.
+    rewrite -[eval _ _ _ = ⊤]predicate_not_empty_iff_full. 2: auto.
     
     (*
         (* TODO: I would like to simplify the RHS, but cannot find a way. *)
@@ -598,7 +598,7 @@ Section semantics.
     rewrite -> Not_Empty_iff_Contains_Elements.
     split.
     - intros [x0 Hx0].
-      rewrite -> pattern_interpretation_ex_simpl in Hx0.
+      rewrite -> eval_ex_simpl in Hx0.
       simpl in Hx0. unfold propset_fa_union in Hx0. rewrite -> elem_of_PropSet in Hx0.
       destruct Hx0 as [c Hc].
       exists c.
@@ -610,18 +610,18 @@ Section semantics.
       apply Not_Empty_iff_Contains_Elements in Hm.
       destruct Hm as [x0 Hx0].
       exists x0.
-      rewrite pattern_interpretation_ex_simpl. simpl.
+      rewrite eval_ex_simpl. simpl.
       unfold propset_fa_union. rewrite -> elem_of_PropSet.
       exists m. assumption.
   Qed.
 
-  Lemma pattern_interpretation_exists_empty M ϕ ρₑ ρ :
+  Lemma eval_exists_empty M ϕ ρₑ ρ :
     let x := fresh_evar ϕ in
-    pattern_interpretation ρₑ ρ (patt_exists ϕ) = ∅ <->
-    ∀ (m : Domain M), pattern_interpretation (update_evar_val x m ρₑ) ρ (evar_open 0 x ϕ) = ∅.
+    eval ρₑ ρ (patt_exists ϕ) = ∅ <->
+    ∀ (m : Domain M), eval (update_evar_val x m ρₑ) ρ (evar_open 0 x ϕ) = ∅.
   Proof.
     intros x.
-    rewrite -> pattern_interpretation_ex_simpl. simpl.
+    rewrite -> eval_ex_simpl. simpl.
     rewrite -> set_eq_subseteq.
     split.
     - intros [H1 _] m.
@@ -655,7 +655,7 @@ Section semantics.
   
   Definition satisfies_model (m : Model) (phi : Pattern) : Prop :=
     forall (evar_val : evar -> Domain m) (svar_val : svar -> propset (Domain m)),
-      pattern_interpretation (m := m) evar_val svar_val phi = Full.
+      eval (m := m) evar_val svar_val phi = Full.
 
   Definition satisfies_theory (m : Model) (theory : Theory)
     : Prop := forall axiom : Pattern, axiom ∈ theory -> (satisfies_model m axiom).
@@ -730,17 +730,17 @@ Section semantics.
 
 
   (* If phi1 \subseteq phi2, then U_x phi1 \subseteq U_x phi2 *)
-  Lemma pattern_interpretation_subset_union M x phi1 phi2 :
+  Lemma eval_subset_union M x phi1 phi2 :
     (forall evar_val svar_val,
-        (@pattern_interpretation M evar_val svar_val phi1)
-          ⊆ (pattern_interpretation evar_val svar_val phi2)
+        (@eval M evar_val svar_val phi1)
+          ⊆ (eval evar_val svar_val phi2)
     )
     -> (forall evar_val svar_val,
-                    (propset_fa_union (fun e => pattern_interpretation (update_evar_val x e evar_val)
+                    (propset_fa_union (fun e => eval (update_evar_val x e evar_val)
                                                                svar_val
                                                                phi1))
                     ⊆
-                    (propset_fa_union (fun e => @pattern_interpretation M (update_evar_val x e evar_val)
+                    (propset_fa_union (fun e => @eval M (update_evar_val x e evar_val)
                                                                svar_val
                                                                phi2))
        ).
@@ -748,57 +748,57 @@ Section semantics.
     intros H. induction phi1; intros; apply propset_fa_union_included; auto.
   Qed.
 
-  (* pattern_interpretation unchanged when using fresh element varaiable *)
-  Lemma Private_pattern_interpretation_free_evar_independent M ρₑ ρ x v sz ϕ:
+  (* eval unchanged when using fresh element varaiable *)
+  Lemma Private_eval_free_evar_independent M ρₑ ρ x v sz ϕ:
     size ϕ <= sz ->
     evar_is_fresh_in x ϕ ->
-    @pattern_interpretation M (update_evar_val x v ρₑ) ρ ϕ
-    = @pattern_interpretation M ρₑ ρ ϕ.
+    @eval M (update_evar_val x v ρₑ) ρ ϕ
+    = @eval M ρₑ ρ ϕ.
   Proof.
     generalize dependent v. generalize dependent x.
     generalize dependent ρ. generalize dependent ρₑ. generalize dependent ϕ.
     induction sz; intros ϕ ρₑ ρ x v; destruct ϕ; simpl; intros Hsz Hnotin; unfold evar_is_fresh_in in Hnotin;
       simpl in Hnotin.
-    - repeat rewrite -> pattern_interpretation_free_evar_simpl.
+    - repeat rewrite -> eval_free_evar_simpl.
       apply f_equal. unfold update_evar_val.
       destruct (decide (x = x0)); simpl.
       + subst.
         apply not_elem_of_singleton_1 in Hnotin.
         contradiction.
       + reflexivity.
-    - repeat rewrite -> pattern_interpretation_free_svar_simpl.
+    - repeat rewrite -> eval_free_svar_simpl.
       reflexivity.
-    - repeat rewrite -> pattern_interpretation_bound_evar_simpl.
+    - repeat rewrite -> eval_bound_evar_simpl.
       reflexivity.
-    - repeat rewrite -> pattern_interpretation_bound_svar_simpl.
+    - repeat rewrite -> eval_bound_svar_simpl.
       reflexivity.
-    - repeat rewrite -> pattern_interpretation_sym_simpl.
-      reflexivity.
-    - lia.
-    - repeat rewrite -> pattern_interpretation_bott_simpl.
+    - repeat rewrite -> eval_sym_simpl.
       reflexivity.
     - lia.
+    - repeat rewrite -> eval_bott_simpl.
+      reflexivity.
     - lia.
     - lia.
+    - lia.
     - apply IHsz. 2: { simpl. apply Hnotin. } simpl. lia.
     - apply IHsz. 2: { simpl. apply Hnotin. } simpl. lia.
     - apply IHsz. 2: { simpl. apply Hnotin. } simpl. lia.
     - apply IHsz. 2: { simpl. apply Hnotin. } simpl. lia.
     - apply IHsz. 2: { simpl. apply Hnotin. } simpl. lia.
-    - repeat rewrite -> pattern_interpretation_app_simpl.
+    - repeat rewrite -> eval_app_simpl.
       simpl in Hnotin.
       apply not_elem_of_union in Hnotin. destruct Hnotin as [Hnotin1 Hnotin2].
       rewrite -> IHsz. 3: apply Hnotin1. 2: lia.
       rewrite -> IHsz. 3: apply Hnotin2. 2: lia.
       reflexivity.
     - apply IHsz. 2: { simpl. apply Hnotin. } simpl. lia.
-    - repeat rewrite -> pattern_interpretation_imp_simpl.
+    - repeat rewrite -> eval_imp_simpl.
       simpl in Hnotin.
       apply not_elem_of_union in Hnotin. destruct Hnotin as [Hnotin1 Hnotin2].
       rewrite -> IHsz. 3: apply Hnotin1. 2: lia.
       rewrite -> IHsz. 3: apply Hnotin2. 2: lia.
       reflexivity.
-    - repeat rewrite -> pattern_interpretation_ex_simpl.
+    - repeat rewrite -> eval_ex_simpl.
       simpl.
       
       apply f_equal. apply functional_extensionality. intros e.
@@ -817,7 +817,7 @@ Section semantics.
         }
         2: { rewrite <- evar_open_size. lia. }
         reflexivity.
-    - repeat rewrite -> pattern_interpretation_mu_simpl. simpl.
+    - repeat rewrite -> eval_mu_simpl. simpl.
       
       apply f_equal. apply functional_extensionality.
       intros e.
@@ -832,75 +832,75 @@ Section semantics.
       reflexivity.
   Qed.
 
-  Lemma pattern_interpretation_free_evar_independent M ρₑ ρₛ x v ϕ:
+  Lemma eval_free_evar_independent M ρₑ ρₛ x v ϕ:
     evar_is_fresh_in x ϕ ->
-    @pattern_interpretation M (update_evar_val x v ρₑ) ρₛ ϕ
-    = @pattern_interpretation M ρₑ ρₛ ϕ.
+    @eval M (update_evar_val x v ρₑ) ρₛ ϕ
+    = @eval M ρₑ ρₛ ϕ.
   Proof.
     intros.
-    apply Private_pattern_interpretation_free_evar_independent with (sz := size ϕ).
+    apply Private_eval_free_evar_independent with (sz := size ϕ).
     * lia.
     * assumption.
   Qed.
 
-  (* pattern_interpretation unchanged when using fresh set varaiable *)
-  Lemma Private_pattern_interpretation_free_svar_independent M ρₑ ρₛ X S sz ϕ:
+  (* eval unchanged when using fresh set varaiable *)
+  Lemma Private_eval_free_svar_independent M ρₑ ρₛ X S sz ϕ:
     size ϕ <= sz ->
     svar_is_fresh_in X ϕ ->
-    @pattern_interpretation M ρₑ (update_svar_val X S ρₛ) ϕ
-    = @pattern_interpretation M ρₑ ρₛ ϕ.
+    @eval M ρₑ (update_svar_val X S ρₛ) ϕ
+    = @eval M ρₑ ρₛ ϕ.
   Proof.
     generalize dependent S. generalize dependent X.
     generalize dependent ρₛ. generalize dependent ρₑ. generalize dependent ϕ.
     induction sz; intros ϕ ρₑ ρₛ X S; destruct ϕ; simpl; intros Hsz Hnotin; unfold svar_is_fresh_in in Hnotin;
       simpl in Hnotin.
-    - repeat rewrite -> pattern_interpretation_free_evar_simpl.
+    - repeat rewrite -> eval_free_evar_simpl.
       reflexivity.
-    - repeat rewrite pattern_interpretation_free_svar_simpl.
+    - repeat rewrite eval_free_svar_simpl.
       unfold update_svar_val.
       destruct (decide (X = x)); simpl.
       + subst.
         apply not_elem_of_singleton_1 in Hnotin.
         contradiction.
       + reflexivity.
-    - repeat rewrite -> pattern_interpretation_free_svar_simpl.
+    - repeat rewrite -> eval_free_svar_simpl.
       reflexivity.
-    - repeat rewrite -> pattern_interpretation_bound_evar_simpl.
+    - repeat rewrite -> eval_bound_evar_simpl.
       reflexivity.
-    - repeat rewrite -> pattern_interpretation_bound_svar_simpl.
-      reflexivity.
-    - lia.
-    - repeat rewrite -> pattern_interpretation_bott_simpl.
+    - repeat rewrite -> eval_bound_svar_simpl.
       reflexivity.
     - lia.
+    - repeat rewrite -> eval_bott_simpl.
+      reflexivity.
     - lia.
     - lia.
+    - lia.
     - apply IHsz. 2: { simpl. apply Hnotin. } simpl. lia.
     - apply IHsz. 2: { simpl. apply Hnotin. } simpl. lia.
     - apply IHsz. 2: { simpl. apply Hnotin. } simpl. lia.
     - apply IHsz. 2: { simpl. apply Hnotin. } simpl. lia.
     - apply IHsz. 2: { simpl. apply Hnotin. } simpl. lia.
-    - repeat rewrite -> pattern_interpretation_app_simpl.
+    - repeat rewrite -> eval_app_simpl.
       simpl in Hnotin.
       apply not_elem_of_union in Hnotin. destruct Hnotin as [Hnotin1 Hnotin2].
       rewrite -> IHsz. 3: apply Hnotin1. 2: lia.
       rewrite -> IHsz. 3: apply Hnotin2. 2: lia.
       reflexivity.
     - apply IHsz. 2: { simpl. apply Hnotin. } simpl. lia.
-    - repeat rewrite -> pattern_interpretation_imp_simpl.
+    - repeat rewrite -> eval_imp_simpl.
       simpl in Hnotin.
       apply not_elem_of_union in Hnotin. destruct Hnotin as [Hnotin1 Hnotin2].
       rewrite -> IHsz. 3: apply Hnotin1. 2: lia.
       rewrite -> IHsz. 3: apply Hnotin2. 2: lia.
       reflexivity.
-    - repeat rewrite -> pattern_interpretation_ex_simpl.
+    - repeat rewrite -> eval_ex_simpl.
       simpl.
       apply f_equal. apply functional_extensionality. intros e.
       rewrite IHsz.
       { rewrite -evar_open_size. lia. }
       { apply svar_fresh_evar_open. apply Hnotin. }
       reflexivity.
-    - repeat rewrite pattern_interpretation_mu_simpl. simpl.
+    - repeat rewrite eval_mu_simpl. simpl.
       apply f_equal. apply functional_extensionality.
       intros e.
       destruct (decide ((fresh_svar ϕ) = X)).
@@ -922,33 +922,33 @@ Section semantics.
         reflexivity.
   Qed.
 
-  Lemma pattern_interpretation_free_svar_independent M ρₑ ρ X S ϕ:
+  Lemma eval_free_svar_independent M ρₑ ρ X S ϕ:
     svar_is_fresh_in X ϕ ->
-    @pattern_interpretation M ρₑ (update_svar_val X S ρ) ϕ
-    = @pattern_interpretation M ρₑ ρ ϕ.
+    @eval M ρₑ (update_svar_val X S ρ) ϕ
+    = @eval M ρₑ ρ ϕ.
   Proof.
     intros.
-    apply Private_pattern_interpretation_free_svar_independent with (sz := size ϕ).
+    apply Private_eval_free_svar_independent with (sz := size ϕ).
     * lia.
     * assumption.
   Qed.
 
   (* Can change updated/opened fresh variable variable *)
-  Lemma Private_interpretation_fresh_var_open M sz ϕ dbi ρₑ ρ:
+  Lemma Private_eval_fresh_var_open M sz ϕ dbi ρₑ ρ:
     size ϕ <= sz ->
     (
       forall X Y S,
         svar_is_fresh_in X ϕ ->
         svar_is_fresh_in Y ϕ ->
-        @pattern_interpretation M ρₑ (update_svar_val X S ρ) (svar_open dbi X ϕ)
-        = @pattern_interpretation M ρₑ (update_svar_val Y S ρ) (svar_open dbi Y ϕ)
+        @eval M ρₑ (update_svar_val X S ρ) (svar_open dbi X ϕ)
+        = @eval M ρₑ (update_svar_val Y S ρ) (svar_open dbi Y ϕ)
     ) /\
     (
       forall x y c,
         evar_is_fresh_in x ϕ ->
         evar_is_fresh_in y ϕ ->
-        @pattern_interpretation M (update_evar_val x c ρₑ) ρ (evar_open dbi x ϕ)
-        = @pattern_interpretation M (update_evar_val y c ρₑ) ρ (evar_open dbi y ϕ)
+        @eval M (update_evar_val x c ρₑ) ρ (evar_open dbi x ϕ)
+        = @eval M (update_evar_val y c ρₑ) ρ (evar_open dbi y ϕ)
     )
   .
   Proof.
@@ -960,51 +960,51 @@ Section semantics.
         (* base case - svar *)
         move=> X Y S HfrX HfrY.
         destruct ϕ; simpl in Hsz; try lia.
-        + rewrite 2!pattern_interpretation_free_evar_simpl. reflexivity.
-        + rewrite 2!pattern_interpretation_free_svar_simpl.
+        + rewrite 2!eval_free_evar_simpl. reflexivity.
+        + rewrite 2!eval_free_svar_simpl.
           unfold svar_is_fresh_in in HfrX, HfrY. simpl in HfrX, HfrY.
           apply not_elem_of_singleton_1 in HfrX.
           apply not_elem_of_singleton_1 in HfrY.
           unfold update_svar_val.
           destruct (decide (X = x)),(decide (Y = x)); simpl; try contradiction.
           reflexivity.
-        + rewrite 2!pattern_interpretation_bound_evar_simpl. reflexivity.
+        + rewrite 2!eval_bound_evar_simpl. reflexivity.
         + unfold svar_open. simpl. case_match.
-          * rewrite 2!pattern_interpretation_bound_svar_simpl.
+          * rewrite 2!eval_bound_svar_simpl.
             reflexivity.
-          * rewrite 2!pattern_interpretation_free_svar_simpl.
+          * rewrite 2!eval_free_svar_simpl.
             rewrite 2!update_svar_val_same. reflexivity.
-          * rewrite 2!pattern_interpretation_bound_svar_simpl.
+          * rewrite 2!eval_bound_svar_simpl.
             reflexivity.
-        + rewrite 2!pattern_interpretation_sym_simpl.
+        + rewrite 2!eval_sym_simpl.
           reflexivity.
-        + rewrite 2!pattern_interpretation_bott_simpl.
+        + rewrite 2!eval_bott_simpl.
           reflexivity.
       }
       {
         (* base case - evar *)
         move=> x y c Hfrx Hfry.
         destruct ϕ; simpl in Hsz; try lia.
-        + rewrite 2!pattern_interpretation_free_evar_simpl.
+        + rewrite 2!eval_free_evar_simpl.
           unfold evar_is_fresh_in in Hfrx, Hfry. simpl in Hfrx, Hfry.
           apply not_elem_of_singleton_1 in Hfrx.
           apply not_elem_of_singleton_1 in Hfry.
           apply f_equal. unfold update_evar_val.
           destruct (decide (x = x0)),(decide (y = x0)); simpl; try contradiction.
           reflexivity.
-        + rewrite 2!pattern_interpretation_free_svar_simpl.
+        + rewrite 2!eval_free_svar_simpl.
           reflexivity.
         + unfold evar_open. simpl. case_match.
-          * rewrite 2!pattern_interpretation_bound_evar_simpl.
+          * rewrite 2!eval_bound_evar_simpl.
             reflexivity.
-          * rewrite 2!pattern_interpretation_free_evar_simpl.
+          * rewrite 2!eval_free_evar_simpl.
             rewrite 2!update_evar_val_same. reflexivity.
-          * rewrite 2!pattern_interpretation_bound_evar_simpl.
+          * rewrite 2!eval_bound_evar_simpl.
             reflexivity.
-        + rewrite 2!pattern_interpretation_bound_svar_simpl. reflexivity.
-        + rewrite 2!pattern_interpretation_sym_simpl.
+        + rewrite 2!eval_bound_svar_simpl. reflexivity.
+        + rewrite 2!eval_sym_simpl.
           reflexivity.
-        + rewrite 2!pattern_interpretation_bott_simpl.
+        + rewrite 2!eval_bott_simpl.
           reflexivity.
       }
     - move=> ϕ dbi ρₑ ρ Hsz.
@@ -1018,7 +1018,7 @@ Section semantics.
         + rewrite (proj1 (IHsz _ _ _ _ _) X Y). 4: reflexivity. 3,2: auto. simpl. lia.
         + rewrite (proj1 (IHsz _ _ _ _ _) X Y). 4: reflexivity. 3,2: auto. simpl. lia.
         + rewrite (proj1 (IHsz _ _ _ _ _) X Y). 4: reflexivity. 3,2: auto. simpl. lia.
-        + rewrite 2!pattern_interpretation_app_simpl. fold svar_open.
+        + rewrite 2!eval_app_simpl. fold svar_open.
           rewrite (proj1 (IHsz _ _ _ _ _) X Y). 4: rewrite (proj1 (IHsz _ _ _ _ _) X Y). lia.
           eapply svar_is_fresh_in_app_l. apply HfrX.
           eapply svar_is_fresh_in_app_l. apply HfrY.
@@ -1027,7 +1027,7 @@ Section semantics.
           eapply svar_is_fresh_in_app_r. apply HfrY.
           reflexivity.
         + rewrite (proj1 (IHsz _ _ _ _ _) X Y). 4: reflexivity. 3,2: auto. simpl. lia.
-        + rewrite 2!pattern_interpretation_imp_simpl. fold svar_open.
+        + rewrite 2!eval_imp_simpl. fold svar_open.
           rewrite (proj1 (IHsz _ _ _ _ _) X Y). 4: rewrite (proj1 (IHsz _ _ _ _ _) X Y). lia.
           eapply svar_is_fresh_in_app_l. apply HfrX.
           eapply svar_is_fresh_in_app_l. apply HfrY.
@@ -1035,7 +1035,7 @@ Section semantics.
           eapply svar_is_fresh_in_app_r. apply HfrX.
           eapply svar_is_fresh_in_app_r. apply HfrY.
           reflexivity.
-        + rewrite 2!pattern_interpretation_ex_simpl. fold svar_open. simpl.
+        + rewrite 2!eval_ex_simpl. fold svar_open. simpl.
           apply f_equal. apply functional_extensionality. intros e.
           rewrite 2!svar_open_evar_open_comm.
           rewrite (proj1 (IHsz _ _ _ _ _) X Y). rewrite -evar_open_size. lia.
@@ -1050,7 +1050,7 @@ Section semantics.
           apply set_evar_fresh_is_fresh.
           reflexivity.
         + rewrite 2!svar_open_mu.
-          rewrite 2!pattern_interpretation_mu_simpl. fold svar_open. simpl.
+          rewrite 2!eval_mu_simpl. fold svar_open. simpl.
           apply f_equal. apply functional_extensionality.
           intros S'.
 
@@ -1128,7 +1128,7 @@ Section semantics.
         + rewrite (proj2 (IHsz _ _ _ _ _) x y). 4: reflexivity. 3,2: auto. simpl. lia.
         + rewrite (proj2 (IHsz _ _ _ _ _) x y). 4: reflexivity. 3,2: auto. simpl. lia.
         + rewrite (proj2 (IHsz _ _ _ _ _) x y). 4: reflexivity. 3,2: auto. simpl. lia.
-        + rewrite 2!pattern_interpretation_app_simpl. fold evar_open.
+        + rewrite 2!eval_app_simpl. fold evar_open.
           rewrite (proj2 (IHsz _ _ _ _ _) x y). 4: rewrite (proj2 (IHsz _ _ _ _ _) x y). lia.
           eapply evar_is_fresh_in_app_l. apply Hfrx.
           eapply evar_is_fresh_in_app_l. apply Hfry.
@@ -1137,7 +1137,7 @@ Section semantics.
           eapply evar_is_fresh_in_app_r. apply Hfry.
           reflexivity.
         + rewrite (proj2 (IHsz _ _ _ _ _) x y). 4: reflexivity. 3,2: auto. simpl. lia.
-        + rewrite 2!pattern_interpretation_imp_simpl. fold evar_open.
+        + rewrite 2!eval_imp_simpl. fold evar_open.
           rewrite (proj2 (IHsz _ _ _ _ _) x y). 4: rewrite (proj2 (IHsz _ _ _ _ _) x y). lia.
           eapply evar_is_fresh_in_app_l. apply Hfrx.
           eapply evar_is_fresh_in_app_l. apply Hfry.
@@ -1146,7 +1146,7 @@ Section semantics.
           eapply evar_is_fresh_in_app_r. apply Hfry.
           reflexivity.
         + do 2 rewrite evar_open_exists.
-          rewrite 2!pattern_interpretation_ex_simpl. fold evar_open. simpl.
+          rewrite 2!eval_ex_simpl. fold evar_open. simpl.
           apply f_equal. apply functional_extensionality. intros e.
           remember (fresh_evar (evar_open (Datatypes.S dbi) x ϕ)) as x'.
           remember (fresh_evar (evar_open (Datatypes.S dbi) y ϕ)) as y'.
@@ -1210,7 +1210,7 @@ Section semantics.
           apply evar_open_fresh_notin.
           apply Hfry. apply HnotinFree. intros Contra. symmetry in Contra. contradiction.
           reflexivity.
-        + rewrite 2!pattern_interpretation_mu_simpl. fold evar_open. simpl.
+        + rewrite 2!eval_mu_simpl. fold evar_open. simpl.
           apply f_equal. apply functional_extensionality.
           intros S'.
           rewrite -2!svar_open_evar_open_comm.
@@ -1229,25 +1229,25 @@ Section semantics.
   Qed.
 
 
-  Lemma interpretation_fresh_evar_open M ϕ x y c dbi ρₑ ρ:
+  Lemma eval_fresh_evar_open M ϕ x y c dbi ρₑ ρ:
     evar_is_fresh_in x ϕ ->
     evar_is_fresh_in y ϕ ->
-    @pattern_interpretation M (update_evar_val x c ρₑ) ρ (evar_open dbi x ϕ)
-    = @pattern_interpretation M (update_evar_val y c ρₑ) ρ (evar_open dbi y ϕ).
+    @eval M (update_evar_val x c ρₑ) ρ (evar_open dbi x ϕ)
+    = @eval M (update_evar_val y c ρₑ) ρ (evar_open dbi y ϕ).
   Proof.
     move=> Hfrx Hfry.
-    eapply (proj2 (@Private_interpretation_fresh_var_open M (size ϕ) ϕ dbi ρₑ ρ _) x y c); assumption.
+    eapply (proj2 (@Private_eval_fresh_var_open M (size ϕ) ϕ dbi ρₑ ρ _) x y c); assumption.
     Unshelve. lia.
   Qed.
 
-  Lemma interpretation_fresh_svar_open M ϕ X Y S dbi ρₑ ρ:
+  Lemma eval_fresh_svar_open M ϕ X Y S dbi ρₑ ρ:
     svar_is_fresh_in X ϕ ->
     svar_is_fresh_in Y ϕ ->
-    @pattern_interpretation M ρₑ (update_svar_val X S ρ) (svar_open dbi X ϕ)
-    = @pattern_interpretation M ρₑ (update_svar_val Y S ρ) (svar_open dbi Y ϕ).
+    @eval M ρₑ (update_svar_val X S ρ) (svar_open dbi X ϕ)
+    = @eval M ρₑ (update_svar_val Y S ρ) (svar_open dbi Y ϕ).
   Proof.
     move=> HfrX HfrY.
-    eapply (proj1 (@Private_interpretation_fresh_var_open M (size ϕ) ϕ dbi ρₑ ρ _) X Y S); assumption.
+    eapply (proj1 (@Private_eval_fresh_var_open M (size ϕ) ϕ dbi ρₑ ρ _) X Y S); assumption.
     Unshelve. lia.
   Qed.
 
@@ -1260,38 +1260,38 @@ Section semantics.
                                 (svar_val : SVarVal) (X : svar),
         well_formed_closed phi2 -> well_formed_closed_mu_aux phi1 (S dbi) ->
         ~ elem_of X (free_svars phi1) ->
-        @pattern_interpretation M evar_val svar_val (bsvar_subst phi1 phi2 dbi)
-        = @pattern_interpretation M evar_val
-                                  (update_svar_val X (@pattern_interpretation M evar_val svar_val phi2) svar_val)
+        @eval M evar_val svar_val (bsvar_subst phi1 phi2 dbi)
+        = @eval M evar_val
+                                  (update_svar_val X (@eval M evar_val svar_val phi2) svar_val)
                                   (svar_open dbi X phi1).
   Proof.
     induction sz; intros dbi M phi1 phi2 Hsz evar_val svar_val X Hwfc2 Hwfphi1 H.
     - (* sz == 0 *)
       destruct phi1; simpl in Hsz; simpl.
       + (* free_evar *)
-        repeat rewrite -> pattern_interpretation_free_evar_simpl. auto.
+        repeat rewrite -> eval_free_evar_simpl. auto.
       + (* free_svar *)
         unfold svar_open. simpl.
-        do 2 rewrite -> pattern_interpretation_free_svar_simpl.
+        do 2 rewrite -> eval_free_svar_simpl.
         unfold update_svar_val. destruct (decide (X = x)).
         * simpl in H. simpl. unfold not in H. exfalso. apply H.
           apply elem_of_singleton_2. auto.
         * auto.
       + (* bound_evar *)
-        rewrite 2!pattern_interpretation_bound_evar_simpl.
+        rewrite 2!eval_bound_evar_simpl.
         reflexivity.
       + (* bound_svar *)
         unfold svar_open. simpl.  case_match; simpl.
-        * repeat rewrite -> pattern_interpretation_bound_svar_simpl; auto.
-        * rewrite pattern_interpretation_free_svar_simpl. unfold update_svar_val.
+        * repeat rewrite -> eval_bound_svar_simpl; auto.
+        * rewrite eval_free_svar_simpl. unfold update_svar_val.
           destruct (decide (X = X)). auto. contradiction.
-        * repeat rewrite -> pattern_interpretation_bound_svar_simpl; auto.
+        * repeat rewrite -> eval_bound_svar_simpl; auto.
       + (* sym *)
-        simpl. repeat rewrite -> pattern_interpretation_sym_simpl; auto.
+        simpl. repeat rewrite -> eval_sym_simpl; auto.
       + (* app *)
         lia.
       + (* bot *)
-        simpl. repeat rewrite pattern_interpretation_bott_simpl; auto.
+        simpl. repeat rewrite eval_bott_simpl; auto.
       + (* impl *)
         lia.
       + (* ex *)
@@ -1302,29 +1302,29 @@ Section semantics.
       destruct phi1; simpl.
       (* HERE we duplicate some of the effort. I do not like it. *)
       + (* free_evar *)
-        repeat rewrite pattern_interpretation_free_evar_simpl. auto.
+        repeat rewrite eval_free_evar_simpl. auto.
       + (* free_svar *)
         unfold svar_open. simpl.
-        do 2 rewrite -> pattern_interpretation_free_svar_simpl.
+        do 2 rewrite -> eval_free_svar_simpl.
         unfold update_svar_val. destruct (decide (X = x)).
         * simpl in H. simpl. unfold not in H. exfalso. apply H.
           apply elem_of_singleton_2. auto.
         * auto.
       + (* bound_evar *)
-        rewrite !pattern_interpretation_bound_evar_simpl. reflexivity.
+        rewrite !eval_bound_evar_simpl. reflexivity.
       + (* bound_svar *)
         unfold svar_open. simpl. case_match.
-        * repeat rewrite -> pattern_interpretation_bound_evar_simpl; auto.
-        * rewrite pattern_interpretation_free_svar_simpl. unfold update_svar_val.
+        * repeat rewrite -> eval_bound_evar_simpl; auto.
+        * rewrite eval_free_svar_simpl. unfold update_svar_val.
           destruct (decide (X = X)). simpl. auto. contradiction.
-        * repeat rewrite -> pattern_interpretation_bound_svar_simpl; auto.
+        * repeat rewrite -> eval_bound_svar_simpl; auto.
       + (* sym *)
-        simpl. repeat rewrite -> pattern_interpretation_sym_simpl; auto.
+        simpl. repeat rewrite -> eval_sym_simpl; auto.
       (* HERE the duplication ends *)
       + (* app *) unfold svar_open in *.
         simpl.
         simpl in H. apply not_elem_of_union in H. destruct H.
-        do 2 rewrite -> pattern_interpretation_app_simpl.
+        do 2 rewrite -> eval_app_simpl.
         simpl in Hsz.
         rewrite <- (IHsz _ _ phi1_1), <- (IHsz _ _ phi1_2).
         * reflexivity.
@@ -1337,12 +1337,12 @@ Section semantics.
         * now apply andb_true_iff in Hwfphi1.
         * auto.
       + (* Bot. Again, a duplication of the sz=0 case *)
-        simpl. repeat rewrite pattern_interpretation_bott_simpl; auto.
+        simpl. repeat rewrite eval_bott_simpl; auto.
       + (* imp *)
         unfold svar_open in *.
         simpl in Hsz. simpl in H. simpl.
         apply not_elem_of_union in H. destruct H.
-        do 2 rewrite -> pattern_interpretation_imp_simpl.
+        do 2 rewrite -> eval_imp_simpl.
         rewrite <- IHsz, <- IHsz.
         * reflexivity.
         * lia.
@@ -1355,7 +1355,7 @@ Section semantics.
         * auto.
 
       + simpl in Hsz. simpl in H. unfold svar_open in *. simpl.
-        do 2 rewrite -> pattern_interpretation_ex_simpl. simpl.
+        do 2 rewrite -> eval_ex_simpl. simpl.
         apply propset_fa_union_same. intros c.
 
         (* x = fresh_evar phi1' *)
@@ -1364,8 +1364,8 @@ Section semantics.
         remember (bsvar_subst phi1 (patt_free_svar X) dbi) as phi1'.
         remember (fresh_evar phi1') as Xfr2'.
         remember (evar_fresh (elements (union (free_evars phi1') (free_evars phi2)))) as Xu.
-        remember (update_svar_val X (pattern_interpretation evar_val svar_val phi2) svar_val) as svar_val2'.
-        pose proof (Hfresh_subst := @interpretation_fresh_evar_open M phi1' Xfr2' Xu c 0 evar_val svar_val2').
+        remember (update_svar_val X (eval evar_val svar_val phi2) svar_val) as svar_val2'.
+        pose proof (Hfresh_subst := @eval_fresh_evar_open M phi1' Xfr2' Xu c 0 evar_val svar_val2').
 
         rewrite -> Hfresh_subst.
         2: { subst Xfr2'. apply set_evar_fresh_is_fresh. }
@@ -1392,14 +1392,14 @@ Section semantics.
           pose proof (HXfr1Fresh2 := evar_fresh_in_subformula Hsub HXfr1Fresh).
 
           assert (Hinterp:
-                    (pattern_interpretation evar_val1' svar_val phi2) =
-                    (pattern_interpretation evar_val svar_val phi2)
+                    (eval evar_val1' svar_val phi2) =
+                    (eval evar_val svar_val phi2)
                  ).
-          { subst. apply pattern_interpretation_free_evar_independent. auto. }
+          { subst. apply eval_free_evar_independent. auto. }
           
           assert (He1e1':
-                    (update_svar_val X (pattern_interpretation evar_val1' svar_val phi2) svar_val) =
-                    (update_svar_val X (pattern_interpretation evar_val svar_val phi2) svar_val)
+                    (update_svar_val X (eval evar_val1' svar_val phi2) svar_val) =
+                    (update_svar_val X (eval evar_val svar_val phi2) svar_val)
                  ).
           { congruence. }
           subst svar_val2'.
@@ -1433,9 +1433,9 @@ Section semantics.
             apply svar_open_not_occur with (x:=X) in Hwfphi1 as HWF.
             (* X is not free in phi1, so the fact that in svar_val2' it is updated to some 
            value is irrelevant. *)
-            assert (Hpi: pattern_interpretation evar_val2' svar_val2' (evar_open 0 Xu phi1')
-                         = pattern_interpretation evar_val2' svar_val (evar_open 0 Xu phi1')).
-            { subst svar_val2'. apply pattern_interpretation_free_svar_independent.
+            assert (Hpi: eval evar_val2' svar_val2' (evar_open 0 Xu phi1')
+                         = eval evar_val2' svar_val (evar_open 0 Xu phi1')).
+            { subst svar_val2'. apply eval_free_svar_independent.
               unfold svar_is_fresh_in. rewrite -> free_svars_evar_open. subst phi1'.
               replace (bsvar_subst phi1 (patt_free_svar X) dbi) with
                       (svar_open dbi X phi1) by reflexivity.
@@ -1443,7 +1443,7 @@ Section semantics.
             }
             rewrite -> Hpi. subst phi1'. unfold svar_open in HWF. rewrite -> HWF.
             subst evar_val1'. subst evar_val2'.
-            rewrite -> interpretation_fresh_evar_open with (y := Xu).
+            rewrite -> eval_fresh_evar_open with (y := Xu).
             reflexivity.
             { subst Xfr1.
               symmetry in HeqHoc'.
@@ -1463,7 +1463,7 @@ Section semantics.
 
       + (* Mu case *)
         rewrite svar_open_mu.
-        rewrite 2!pattern_interpretation_mu_simpl. simpl.
+        rewrite 2!eval_mu_simpl. simpl.
         apply f_equal. apply functional_extensionality. intros E.
 
         remember (bsvar_subst phi1 phi2 (S dbi)) as phi_subst.
@@ -1513,7 +1513,7 @@ Section semantics.
         --
           subst phi_subst.
 
-          rewrite (@interpretation_fresh_svar_open _ _ ((fresh_svar (svar_open (S dbi) X phi1))) Y).
+          rewrite (@eval_fresh_svar_open _ _ ((fresh_svar (svar_open (S dbi) X phi1))) Y).
           { apply set_svar_fresh_is_fresh. }
           { apply Hfreshy''. }
 
@@ -1525,9 +1525,9 @@ Section semantics.
 
           remember ((update_svar_val Y E svar_val)) as svar_val'.
 
-          assert (Hpieq: (pattern_interpretation evar_val svar_val' phi2) = (pattern_interpretation evar_val svar_val phi2)).
+          assert (Hpieq: (eval evar_val svar_val' phi2) = (eval evar_val svar_val phi2)).
           { subst svar_val'.
-            apply pattern_interpretation_free_svar_independent.
+            apply eval_free_svar_independent.
             apply Hfreshy''''.
           }
           rewrite -Hpieq.
@@ -1558,7 +1558,7 @@ Section semantics.
           2: { apply Hwfc2. }
           2: { lia. }
           replace (pred (S dbi)) with dbi by lia.
-          apply interpretation_fresh_svar_open.
+          apply eval_fresh_svar_open.
           { subst X'. apply set_svar_fresh_is_fresh. }
           { apply Hfreshy5.  }
           
@@ -1568,7 +1568,7 @@ Section semantics.
           rewrite bsvar_subst_not_occur in Heqphi_subst. all: auto.
           1-2: apply wfc_mu_lower; auto.
 
-          rewrite -> interpretation_fresh_svar_open with (X := fresh_svar phi1) (Y := Y).
+          rewrite -> eval_fresh_svar_open with (X := fresh_svar phi1) (Y := Y).
           2: { apply set_svar_fresh_is_fresh. }
           2: { subst.
                eapply svar_is_fresh_in_richer'.
@@ -1585,16 +1585,16 @@ Section semantics.
 
           destruct (decide (X = (fresh_svar phi1))).
           ++ subst X. rewrite update_svar_val_shadow.
-             apply interpretation_fresh_svar_open.
+             apply eval_fresh_svar_open.
              { apply Hfreshy'. }
              apply set_svar_fresh_is_fresh.
           ++ rewrite update_svar_val_comm.
              { apply not_eq_sym. apply n. }                              
-             rewrite -> pattern_interpretation_free_svar_independent with (X:=X).
+             rewrite -> eval_free_svar_independent with (X:=X).
              2: { apply svar_is_fresh_in_svar_open. apply n.
                   simpl in H. apply H.
              }
-             apply interpretation_fresh_svar_open.
+             apply eval_fresh_svar_open.
              { apply Hfreshy'. }
              apply set_svar_fresh_is_fresh.
   Qed.
@@ -1603,9 +1603,9 @@ Section semantics.
       forall (evar_val : EVarVal) (svar_val : SVarVal) (X : svar),
         well_formed_closed phi2 -> well_formed_closed_mu_aux phi1 (S dbi) ->
         ~ elem_of X (free_svars phi1) ->
-        @pattern_interpretation M evar_val svar_val (bsvar_subst phi1 phi2 dbi)
-        = @pattern_interpretation M evar_val
-                                  (update_svar_val X (@pattern_interpretation M evar_val svar_val phi2) svar_val)
+        @eval M evar_val svar_val (bsvar_subst phi1 phi2 dbi)
+        = @eval M evar_val
+                                  (update_svar_val X (@eval M evar_val svar_val phi2) svar_val)
                                   (svar_open dbi X phi1).
   Proof.
     intros.
@@ -1617,8 +1617,8 @@ Section semantics.
       size phi <= sz -> forall (evar_val : EVarVal)
                                (svar_val : SVarVal) (x : evar),
         evar_is_fresh_in x phi -> well_formed_closed_ex_aux phi (S dbi) ->
-        @pattern_interpretation M evar_val svar_val (bevar_subst phi (patt_free_evar y) dbi)
-        = @pattern_interpretation M
+        @eval M evar_val svar_val (bevar_subst phi (patt_free_evar y) dbi)
+        = @eval M
                                   (update_evar_val x (evar_val y) evar_val)
                                   svar_val
                                   (evar_open dbi x phi).
@@ -1629,31 +1629,31 @@ Section semantics.
       + (* free_evar *)
         unfold evar_is_fresh_in in H.
         rewrite evar_open_free_evar.
-        repeat rewrite -> pattern_interpretation_free_evar_simpl.
+        repeat rewrite -> eval_free_evar_simpl.
         unfold update_evar_val.
         destruct (decide (x = x0)).
         * simpl. unfold not in H. exfalso. apply H.
           apply elem_of_singleton_2. auto.
         * auto.
       + (* free_svar *)
-        repeat rewrite -> pattern_interpretation_free_svar_simpl.
+        repeat rewrite -> eval_free_svar_simpl.
         auto.
       + (* bound_evar *)
         rewrite evar_open_bound_evar.
         case_match; subst.
         * auto.
-        * do 2 rewrite pattern_interpretation_free_evar_simpl.
+        * do 2 rewrite eval_free_evar_simpl.
           unfold update_evar_val.
           case_match; auto. contradiction.
         * auto.
       + (* bound_svar *)
-        rewrite 2!pattern_interpretation_bound_svar_simpl; auto.
+        rewrite 2!eval_bound_svar_simpl; auto.
       + (* sym *)
-        simpl. repeat rewrite -> pattern_interpretation_sym_simpl; auto.
+        simpl. repeat rewrite -> eval_sym_simpl; auto.
       + (* app *)
         lia.
       + (* bot *)
-        simpl. repeat rewrite pattern_interpretation_bott_simpl; auto.
+        simpl. repeat rewrite eval_bott_simpl; auto.
       + (* impl *)
         lia.
       + (* ex *)
@@ -1665,31 +1665,31 @@ Section semantics.
       (* HERE we duplicate some of the effort. I do not like it. *)
       + (* free_evar *)
         unfold evar_is_fresh_in in H. rewrite evar_open_free_evar.
-        do 2 rewrite -> pattern_interpretation_free_evar_simpl.
+        do 2 rewrite -> eval_free_evar_simpl.
         unfold update_evar_val.
         destruct (decide (x = x0)).
         * simpl. unfold not in H. exfalso. apply H.
           apply elem_of_singleton_2. auto.
         * auto.
       + (* free_svar *)
-        repeat rewrite -> pattern_interpretation_free_svar_simpl.
+        repeat rewrite -> eval_free_svar_simpl.
         auto.
       + (* bound_evar *)
         rewrite evar_open_bound_evar.
         case_match.
         * auto.
-        * repeat rewrite pattern_interpretation_free_evar_simpl. unfold update_evar_val.
+        * repeat rewrite eval_free_evar_simpl. unfold update_evar_val.
           destruct (decide (x = x)). auto. contradiction.
         * auto.
       + (* bound_svar *)
-        rewrite 2!pattern_interpretation_bound_svar_simpl; auto.
+        rewrite 2!eval_bound_svar_simpl; auto.
       + (* sym *)
-        simpl. repeat rewrite -> pattern_interpretation_sym_simpl; auto.
+        simpl. repeat rewrite -> eval_sym_simpl; auto.
       (* HERE the duplication ends *)
       + (* app *)
         rewrite evar_open_app.
         unfold evar_is_fresh_in in H. simpl in H. apply not_elem_of_union in H. destruct H.
-        repeat rewrite -> pattern_interpretation_app_simpl.
+        repeat rewrite -> eval_app_simpl.
         simpl in Hsz.
         repeat rewrite <- IHsz.
         * reflexivity.
@@ -1700,12 +1700,12 @@ Section semantics.
         * auto.
         * now apply andb_true_iff in Hwf.
       + (* Bot. Again, a duplication of the sz=0 case *)
-        simpl. repeat rewrite pattern_interpretation_bott_simpl; auto.
+        simpl. repeat rewrite eval_bott_simpl; auto.
       + (* imp *)
         rewrite evar_open_imp.
         simpl in Hsz.
         unfold evar_is_fresh_in in H. simpl in H. apply not_elem_of_union in H. destruct H.
-        repeat rewrite -> pattern_interpretation_imp_simpl.
+        repeat rewrite -> eval_imp_simpl.
         repeat rewrite <- IHsz.
         * reflexivity.
         * lia.
@@ -1719,7 +1719,7 @@ Section semantics.
         rewrite evar_open_exists.
         simpl in Hsz.
         unfold evar_is_fresh_in in H. simpl in H.
-        repeat rewrite -> pattern_interpretation_ex_simpl. simpl.
+        repeat rewrite -> eval_ex_simpl. simpl.
         apply propset_fa_union_same. intros c.
         remember (fresh_evar (bevar_subst phi (patt_free_evar y) (S dbi))) as x'.
         (* rewrite evar_open_bevar_subst_higher.
@@ -1781,7 +1781,7 @@ Section semantics.
             apply union_subseteq_r.
           }
 
-          rewrite -> interpretation_fresh_evar_open with (x := Xfr') (y := yB).
+          rewrite -> eval_fresh_evar_open with (x := Xfr') (y := yB).
           3: { apply HyBfphi'. }
           2: { subst. apply set_evar_fresh_is_fresh. }
           
@@ -1804,7 +1804,7 @@ Section semantics.
           subst evar_val'.
           rewrite <- evar_open_bevar_subst_higher.
           rewrite <- evar_open_bevar_subst_higher.
-          rewrite -> interpretation_fresh_evar_open with (y := yB).
+          rewrite -> eval_fresh_evar_open with (y := yB).
           reflexivity.
 
           { rewrite Heqx'. apply set_evar_fresh_is_fresh. }
@@ -1817,14 +1817,14 @@ Section semantics.
           { apply evar_is_fresh_in_evar_open. apply not_eq_sym. apply HyBx. apply H. }
           { replace (pred (S dbi)) with dbi by lia. apply wfc_mu_aux_body_ex_imp3; auto. lia. }
       + rewrite evar_open_mu.
-        rewrite 2!pattern_interpretation_mu_simpl. simpl.
+        rewrite 2!eval_mu_simpl. simpl.
         apply f_equal. apply functional_extensionality. intros x0.
         (* fold (evar_open dbi y phi). *)
         remember (evar_open dbi x phi) as phi'.
         remember (fresh_svar phi') as Xfr'.
         remember (svar_fresh (elements (free_svars phi'))) as Xu.
         remember (update_evar_val x (evar_val y) evar_val) as evar_val'.
-        pose proof (Hfresh_subst := @interpretation_fresh_svar_open M phi' Xfr' Xu x0 0 evar_val' svar_val).
+        pose proof (Hfresh_subst := @eval_fresh_svar_open M phi' Xfr' Xu x0 0 evar_val' svar_val).
         rewrite -> Hfresh_subst.
         2: { subst Xfr'. apply set_svar_fresh_is_fresh. }
         2: { subst Xu. apply set_svar_fresh_is_fresh'. }
@@ -1882,9 +1882,9 @@ Section semantics.
             (* symmetry in HeqHoc. apply evar_open_not_occur with (x1:=x) in HeqHoc. *)
             (* X is not free in phi1, so the fact that in evar_val' it is updated to some 
            value is irrelevant. *)
-            assert (Hpi: pattern_interpretation evar_val svar_val2' (svar_open 0 Xu phi')
-                         = pattern_interpretation evar_val' svar_val2' (svar_open 0 Xu phi')).
-            { subst evar_val'. rewrite pattern_interpretation_free_evar_independent; auto.
+            assert (Hpi: eval evar_val svar_val2' (svar_open 0 Xu phi')
+                         = eval evar_val' svar_val2' (svar_open 0 Xu phi')).
+            { subst evar_val'. rewrite eval_free_evar_independent; auto.
               unfold evar_is_fresh_in.
               rewrite -> free_evars_svar_open. subst phi'.
               rewrite evar_open_not_occur; auto.
@@ -1893,7 +1893,7 @@ Section semantics.
             rewrite <- Hpi. subst phi'. rewrite evar_open_not_occur; auto.
             { apply wfc_ex_lower; auto. }
             subst svar_val1'. subst svar_val2'.
-            rewrite -> interpretation_fresh_svar_open with (Y := Xu). reflexivity.
+            rewrite -> eval_fresh_svar_open with (Y := Xu). reflexivity.
             { subst Xfr1.
               simpl in Hwf. symmetry in HeqHoc'.
               apply wfc_ex_lower in Hwf; auto.
@@ -1914,8 +1914,8 @@ Section semantics.
   Lemma element_substitution_lemma
         (M : Model) (phi : Pattern) (x y : evar) (evar_val : EVarVal) (svar_val : SVarVal) (dbi : db_index) :
     evar_is_fresh_in x phi -> well_formed_closed_ex_aux phi (S dbi) ->
-    pattern_interpretation evar_val svar_val (bevar_subst phi (patt_free_evar y) dbi)
-    = @pattern_interpretation M
+    eval evar_val svar_val (bevar_subst phi (patt_free_evar y) dbi)
+    = @eval M
                               (update_evar_val x (evar_val y) evar_val)
                               svar_val
                               (evar_open dbi x phi).
@@ -1924,14 +1924,14 @@ Section semantics.
     apply Private_plugging_patterns_bevar_subst with (sz := size phi);auto.
   Qed.
 
-  (* pattern_interpretation unchanged within subformula over fresh element variable *)
-  Lemma interpretation_fresh_evar_subterm M ϕ₁ ϕ₂ c dbi ρₑ ρ :
+  (* eval unchanged within subformula over fresh element variable *)
+  Lemma eval_fresh_evar_subterm M ϕ₁ ϕ₂ c dbi ρₑ ρ :
     is_subformula_of_ind ϕ₁ ϕ₂ ->
-    @pattern_interpretation M (update_evar_val (fresh_evar ϕ₂) c ρₑ) ρ (evar_open dbi (fresh_evar ϕ₂) ϕ₁)
-    = @pattern_interpretation M (update_evar_val (fresh_evar ϕ₁) c ρₑ) ρ (evar_open dbi (fresh_evar ϕ₁) ϕ₁).
+    @eval M (update_evar_val (fresh_evar ϕ₂) c ρₑ) ρ (evar_open dbi (fresh_evar ϕ₂) ϕ₁)
+    = @eval M (update_evar_val (fresh_evar ϕ₁) c ρₑ) ρ (evar_open dbi (fresh_evar ϕ₁) ϕ₁).
   Proof.
     intros Hsub.
-    apply interpretation_fresh_evar_open; auto.
+    apply eval_fresh_evar_open; auto.
     eapply evar_fresh_in_subformula. apply Hsub.
     apply set_evar_fresh_is_fresh.
   Qed.
@@ -1948,7 +1948,7 @@ Section semantics.
     unfold M_predicate.
     intros H ρₑ ρₛ.
     rewrite -(@update_evar_val_same_2 M x₂ ρₑ).
-    rewrite (@interpretation_fresh_evar_open M _ x₂ x₁); auto.
+    rewrite (@eval_fresh_evar_open M _ x₂ x₁); auto.
   Qed.
 
   Lemma M_predicate_evar_open_fresh_evar_2 M x ϕ :
@@ -1967,23 +1967,23 @@ Section semantics.
    *)
   Lemma Private_free_svar_subst_update_exchange {m : Model}: ∀ sz phi psi X svar_val evar_val,
       le (Pattern.size phi) sz → well_formed psi → well_formed_closed phi → 
-      pattern_interpretation evar_val svar_val (free_svar_subst phi psi X) =
-      pattern_interpretation evar_val
-                             (@update_svar_val m X (pattern_interpretation evar_val svar_val psi) svar_val)
+      eval evar_val svar_val (free_svar_subst phi psi X) =
+      eval evar_val
+                             (@update_svar_val m X (eval evar_val svar_val psi) svar_val)
                              phi.
   Proof.
     unfold free_svar_subst.
     induction sz; destruct phi; intros psi X svar_val evar_val Hsz Hwf Hwfc ; simpl in *; try inversion Hsz; auto.
-    - rewrite -> pattern_interpretation_free_svar_simpl. unfold update_svar_val.
+    - rewrite -> eval_free_svar_simpl. unfold update_svar_val.
       simpl.
       destruct (decide (X = x)); simpl.
       + reflexivity.
-      + rewrite -> pattern_interpretation_free_svar_simpl. reflexivity.
-    -  rewrite -> pattern_interpretation_free_svar_simpl. unfold update_svar_val.
+      + rewrite -> eval_free_svar_simpl. reflexivity.
+    -  rewrite -> eval_free_svar_simpl. unfold update_svar_val.
       destruct (decide (X = x)); simpl.
       + reflexivity.
-      + rewrite -> pattern_interpretation_free_svar_simpl. reflexivity.
-    - repeat rewrite -> pattern_interpretation_app_simpl.
+      + rewrite -> eval_free_svar_simpl. reflexivity.
+    - repeat rewrite -> eval_app_simpl.
       erewrite -> IHsz. erewrite -> IHsz. reflexivity. lia. assumption.
       + apply andb_true_iff in Hwfc as [Hwfc1 Hwfc2]. simpl in Hwfc1, Hwfc2.
         apply andb_true_iff in Hwfc1 as [Hwfc11 Hwfc12].
@@ -1995,19 +1995,7 @@ Section semantics.
         apply andb_true_iff in Hwfc1 as [Hwfc11 Hwfc12].
         apply andb_true_iff in Hwfc2 as [Hwfc21 Hwfc22].
         apply andb_true_iff. split; auto.
-    - repeat rewrite -> pattern_interpretation_app_simpl.
-      erewrite -> IHsz. erewrite -> IHsz. reflexivity. lia. assumption.
-       + apply andb_true_iff in Hwfc as [Hwfc1 Hwfc2]. simpl in Hwfc1, Hwfc2.
-        apply andb_true_iff in Hwfc1 as [Hwfc11 Hwfc12].
-        apply andb_true_iff in Hwfc2 as [Hwfc21 Hwfc22].
-        apply andb_true_iff. split; auto.
-      + lia.
-      + auto.
-      + apply andb_true_iff in Hwfc as [Hwfc1 Hwfc2]. simpl in Hwfc1, Hwfc2.
-        apply andb_true_iff in Hwfc1 as [Hwfc11 Hwfc12].
-        apply andb_true_iff in Hwfc2 as [Hwfc21 Hwfc22].
-        apply andb_true_iff. split; auto.
-    - repeat rewrite -> pattern_interpretation_imp_simpl.
+    - repeat rewrite -> eval_app_simpl.
       erewrite -> IHsz. erewrite -> IHsz. reflexivity. lia. assumption.
        + apply andb_true_iff in Hwfc as [Hwfc1 Hwfc2]. simpl in Hwfc1, Hwfc2.
         apply andb_true_iff in Hwfc1 as [Hwfc11 Hwfc12].
@@ -2019,7 +2007,7 @@ Section semantics.
         apply andb_true_iff in Hwfc1 as [Hwfc11 Hwfc12].
         apply andb_true_iff in Hwfc2 as [Hwfc21 Hwfc22].
         apply andb_true_iff. split; auto.
-    - repeat rewrite -> pattern_interpretation_imp_simpl.
+    - repeat rewrite -> eval_imp_simpl.
       erewrite -> IHsz. erewrite -> IHsz. reflexivity. lia. assumption.
        + apply andb_true_iff in Hwfc as [Hwfc1 Hwfc2]. simpl in Hwfc1, Hwfc2.
         apply andb_true_iff in Hwfc1 as [Hwfc11 Hwfc12].
@@ -2031,7 +2019,19 @@ Section semantics.
         apply andb_true_iff in Hwfc1 as [Hwfc11 Hwfc12].
         apply andb_true_iff in Hwfc2 as [Hwfc21 Hwfc22].
         apply andb_true_iff. split; auto.
-    - repeat rewrite -> pattern_interpretation_ex_simpl. simpl.
+    - repeat rewrite -> eval_imp_simpl.
+      erewrite -> IHsz. erewrite -> IHsz. reflexivity. lia. assumption.
+       + apply andb_true_iff in Hwfc as [Hwfc1 Hwfc2]. simpl in Hwfc1, Hwfc2.
+        apply andb_true_iff in Hwfc1 as [Hwfc11 Hwfc12].
+        apply andb_true_iff in Hwfc2 as [Hwfc21 Hwfc22].
+        apply andb_true_iff. split; auto.
+      + lia.
+      + auto.
+      + apply andb_true_iff in Hwfc as [Hwfc1 Hwfc2]. simpl in Hwfc1, Hwfc2.
+        apply andb_true_iff in Hwfc1 as [Hwfc11 Hwfc12].
+        apply andb_true_iff in Hwfc2 as [Hwfc21 Hwfc22].
+        apply andb_true_iff. split; auto.
+    - repeat rewrite -> eval_ex_simpl. simpl.
       apply propset_fa_union_same. intros.
       rewrite -> set_eq_subseteq.
       repeat rewrite -> elem_of_subseteq.
@@ -2055,7 +2055,7 @@ Section semantics.
         {
           unfold evar_is_fresh_in. assumption.
         }
-        erewrite interpretation_fresh_evar_open in H.
+        erewrite eval_fresh_evar_open in H.
         3: { eassumption. }
         2: { assumption. }
 
@@ -2067,13 +2067,13 @@ Section semantics.
         {
           apply set_evar_fresh_is_fresh.
         }
-        epose (interpretation_fresh_evar_open c 0 evar_val (update_svar_val X (pattern_interpretation evar_val svar_val psi) svar_val) _ _) as HFresh.
+        epose (eval_fresh_evar_open c 0 evar_val (update_svar_val X (eval evar_val svar_val psi) svar_val) _ _) as HFresh.
         rewrite -> HFresh.
         clear HFresh.
         epose (IHsz (evar_open 0 fresh phi) 
                     psi X svar_val 
                     (update_evar_val fresh c evar_val) _ _ ).
-        pose (@pattern_interpretation_free_evar_independent m evar_val svar_val fresh c psi).
+        pose (@eval_free_evar_independent m evar_val svar_val fresh c psi).
         rewrite -> e0 in e. clear e0.
         unfold free_svar_subst in *.
         rewrite -> (@evar_open_free_svar_subst_comm) in H.
@@ -2105,7 +2105,7 @@ Section semantics.
         {
           unfold evar_is_fresh_in. assumption.
         }
-        erewrite -> interpretation_fresh_evar_open.
+        erewrite -> eval_fresh_evar_open.
         3: { eassumption. }
         2: { assumption. }
         assert(evar_is_fresh_in fresh phi).
@@ -2116,13 +2116,13 @@ Section semantics.
         {
           apply set_evar_fresh_is_fresh.
         }
-        epose (interpretation_fresh_evar_open c 0 evar_val (update_svar_val X (pattern_interpretation evar_val svar_val psi) svar_val) _ _) as HFresh.
+        epose (eval_fresh_evar_open c 0 evar_val (update_svar_val X (eval evar_val svar_val psi) svar_val) _ _) as HFresh.
         rewrite -> HFresh in H.
         clear HFresh.
         epose (IHsz (evar_open 0 fresh phi) 
                     psi X svar_val 
                     (update_evar_val fresh c evar_val) _ _ ).
-        pose (@pattern_interpretation_free_evar_independent m evar_val svar_val fresh c psi).
+        pose (@eval_free_evar_independent m evar_val svar_val fresh c psi).
         rewrite -> e0 in e. clear e0. fold free_svar_subst.
         
         rewrite -> (evar_open_free_svar_subst_comm).
@@ -2135,7 +2135,7 @@ Section semantics.
           -- now apply wfc_mu_aux_body_ex_imp1.
           -- now apply wfc_ex_aux_body_ex_imp1.
         * apply andb_true_iff in Hwf as [_ Hwf]. apply andb_true_iff in Hwf as [_ Hwf]. apply Hwf.
-    - repeat rewrite -> pattern_interpretation_ex_simpl. simpl.
+    - repeat rewrite -> eval_ex_simpl. simpl.
       apply propset_fa_union_same. intros.
       rewrite -> set_eq_subseteq.
       repeat rewrite -> elem_of_subseteq.
@@ -2160,7 +2160,7 @@ Section semantics.
           unfold evar_is_fresh_in. assumption.
         }
         
-        epose proof (interpretation_fresh_evar_open c 0 evar_val svar_val
+        epose proof (eval_fresh_evar_open c 0 evar_val svar_val
                                                     H2 H3) as HFresh.
         unfold free_svar_subst in HFresh.
         rewrite -> HFresh in H1.
@@ -2173,13 +2173,13 @@ Section semantics.
         {
           apply set_evar_fresh_is_fresh.
         }
-        epose (interpretation_fresh_evar_open c 0 evar_val (update_svar_val X (pattern_interpretation evar_val svar_val psi) svar_val) _ _) as HFresh.
+        epose (eval_fresh_evar_open c 0 evar_val (update_svar_val X (eval evar_val svar_val psi) svar_val) _ _) as HFresh.
         rewrite -> HFresh.
         clear HFresh.
         epose (IHsz (evar_open 0 fresh phi) 
                     psi X svar_val 
                     (update_evar_val fresh c evar_val) _ _ ).
-        pose (@pattern_interpretation_free_evar_independent m evar_val svar_val fresh c psi).
+        pose (@eval_free_evar_independent m evar_val svar_val fresh c psi).
         rewrite -> e0 in e. clear e0. fold free_svar_subst in H1.
         
         rewrite -> (evar_open_free_svar_subst_comm) in H1.
@@ -2211,7 +2211,7 @@ Section semantics.
         {
           unfold evar_is_fresh_in. assumption.
         }
-        epose (interpretation_fresh_evar_open c 0 evar_val svar_val
+        epose (eval_fresh_evar_open c 0 evar_val svar_val
                                               H2 H3) as HFresh.
         fold free_svar_subst.
         rewrite -> HFresh.
@@ -2224,13 +2224,13 @@ Section semantics.
         {
           apply set_evar_fresh_is_fresh.
         }
-        epose proof (interpretation_fresh_evar_open c 0 evar_val (update_svar_val X (pattern_interpretation evar_val svar_val psi) svar_val) _ _) as HFresh.
+        epose proof (eval_fresh_evar_open c 0 evar_val (update_svar_val X (eval evar_val svar_val psi) svar_val) _ _) as HFresh.
         rewrite -> HFresh in H1.
         clear HFresh.
         epose (IHsz (evar_open 0 fresh phi) 
                     psi X svar_val 
                     (update_evar_val fresh c evar_val) _ _ ).
-        pose (@pattern_interpretation_free_evar_independent m evar_val svar_val fresh c psi).
+        pose (@eval_free_evar_independent m evar_val svar_val fresh c psi).
         rewrite -> e0 in e. clear e0.
         rewrite -> (evar_open_free_svar_subst_comm).
         unfold free_svar_subst.
@@ -2242,15 +2242,15 @@ Section semantics.
           -- now apply wfc_mu_aux_body_ex_imp1.
           -- now apply wfc_ex_aux_body_ex_imp1.
         * apply andb_true_iff in Hwf as [_ Hwf]. apply andb_true_iff in Hwf as [_ Hwf]. apply Hwf.
-    - repeat rewrite -> pattern_interpretation_mu_simpl. simpl.
+    - repeat rewrite -> eval_mu_simpl. simpl.
       assert ((λ S : propset (Domain m),
-                     pattern_interpretation evar_val
+                     eval evar_val
                                             (update_svar_val (fresh_svar (free_svar_subst phi psi X)) S svar_val)
                                             (svar_open 0 (fresh_svar (free_svar_subst phi psi X)) (free_svar_subst phi psi X))) =
               (λ S : propset (Domain m),
-                     pattern_interpretation evar_val
+                     eval evar_val
                                             (update_svar_val (fresh_svar phi) S
-                                                             (update_svar_val X (pattern_interpretation evar_val svar_val psi) svar_val))
+                                                             (update_svar_val X (eval evar_val svar_val psi) svar_val))
                                             (svar_open 0 (fresh_svar phi) phi))).
       apply functional_extensionality. intros.
       + (*Create a common fresh var.*)
@@ -2266,8 +2266,8 @@ Section semantics.
         subst B. apply not_elem_of_union in H. destruct H.
         apply not_elem_of_union in H. destruct H.
         apply not_elem_of_union in H. destruct H.
-        erewrite -> (@interpretation_fresh_svar_open m _ MuX MuZ); try assumption.
-        erewrite -> (@interpretation_fresh_svar_open m _ MuY MuZ); try assumption.
+        erewrite -> (@eval_fresh_svar_open m _ MuX MuZ); try assumption.
+        erewrite -> (@eval_fresh_svar_open m _ MuY MuZ); try assumption.
         erewrite -> svar_open_free_svar_subst_comm; try assumption.
         rewrite update_svar_val_comm; try assumption. 
         {
@@ -2276,7 +2276,7 @@ Section semantics.
         epose (IHsz (svar_open 0 MuZ phi) psi X 
                     (update_svar_val MuZ x svar_val) evar_val _ _ _).
         rewrite e. 
-        erewrite (@pattern_interpretation_free_svar_independent m _ _ MuZ x psi).
+        erewrite (@eval_free_svar_independent m _ _ MuZ x psi).
         reflexivity.
         all: auto.
         {
@@ -2297,15 +2297,15 @@ Section semantics.
         rewrite nest_mu_aux_wfc_mu.
         { unfold well_formed,well_formed_closed in Hwf. destruct_and!. assumption. }
         rewrite H. reflexivity. *)
-    - repeat rewrite -> pattern_interpretation_mu_simpl. simpl.
+    - repeat rewrite -> eval_mu_simpl. simpl.
       assert ((λ S : propset (Domain m),
-                     pattern_interpretation evar_val
+                     eval evar_val
                                             (update_svar_val (fresh_svar (free_svar_subst phi psi X)) S svar_val)
                                             (svar_open 0 (fresh_svar (free_svar_subst phi psi X)) (free_svar_subst phi psi X))) =
               (λ S : propset (Domain m),
-                     pattern_interpretation evar_val
+                     eval evar_val
                                             (update_svar_val (fresh_svar phi) S
-                                                             (update_svar_val X (pattern_interpretation evar_val svar_val psi) svar_val))
+                                                             (update_svar_val X (eval evar_val svar_val psi) svar_val))
                                             (svar_open 0 (fresh_svar phi) phi))).
       apply functional_extensionality. intros.
       + (*Create a common fresh var.*)
@@ -2322,8 +2322,8 @@ Section semantics.
         apply not_elem_of_union in H1. destruct H1.
         apply not_elem_of_union in H1. destruct H1.
         
-        erewrite -> (@interpretation_fresh_svar_open m _ MuX MuZ); try assumption.
-        erewrite -> (@interpretation_fresh_svar_open m _ MuY MuZ); try assumption.
+        erewrite -> (@eval_fresh_svar_open m _ MuX MuZ); try assumption.
+        erewrite -> (@eval_fresh_svar_open m _ MuY MuZ); try assumption.
         erewrite -> svar_open_free_svar_subst_comm; try assumption.
         rewrite update_svar_val_comm; try assumption. 
         {
@@ -2338,7 +2338,7 @@ Section semantics.
           -- now apply wfc_mu_aux_body_mu_imp1.
           -- now apply wfc_ex_aux_body_mu_imp1.
         }
-        erewrite (@pattern_interpretation_free_svar_independent m _ _ MuZ x psi); try assumption.
+        erewrite (@eval_free_svar_independent m _ _ MuZ x psi); try assumption.
         reflexivity.
         unfold well_formed,well_formed_closed in Hwf.
         destruct_and!. all: try assumption.
@@ -2387,9 +2387,9 @@ Section semantics.
 
   Lemma free_svar_subst_update_exchange {m : Model}: ∀ phi psi X svar_val evar_val,
       well_formed psi → well_formed_closed phi → 
-      pattern_interpretation evar_val svar_val (free_svar_subst phi psi X) =
-      pattern_interpretation evar_val (@update_svar_val m X 
-                                                        (pattern_interpretation evar_val svar_val psi) svar_val) 
+      eval evar_val svar_val (free_svar_subst phi psi X) =
+      eval evar_val (@update_svar_val m X 
+                                                        (eval evar_val svar_val psi) svar_val) 
                              phi.
   Proof. 
     intros. apply Private_free_svar_subst_update_exchange with (sz := size phi). 
@@ -2398,26 +2398,26 @@ Section semantics.
 
   (* rho(psi) = empty then C[rho(psi)] = empty *)
   Lemma propagate_context_empty M psi evar_val svar_val C :
-    @pattern_interpretation M evar_val svar_val psi = Empty ->
-    @pattern_interpretation M evar_val svar_val (subst_ctx C psi) = Empty.
+    @eval M evar_val svar_val psi = Empty ->
+    @eval M evar_val svar_val (subst_ctx C psi) = Empty.
   Proof.
     intro Hpsi. induction C.
     * auto.
-    * simpl. rewrite pattern_interpretation_app_simpl. rewrite IHC. apply app_ext_bot_l.
-    * simpl. rewrite pattern_interpretation_app_simpl. rewrite IHC. apply app_ext_bot_r.
+    * simpl. rewrite eval_app_simpl. rewrite IHC. apply app_ext_bot_l.
+    * simpl. rewrite eval_app_simpl. rewrite IHC. apply app_ext_bot_r.
   Qed.
 
   (* application to a singleton *)
   Definition rel_of M ρₑ ρ ϕ: Domain M -> propset (Domain M) :=
     λ m₁,
-    (app_ext (@pattern_interpretation M ρₑ ρ ϕ) {[ m₁ ]}).
+    (app_ext (@eval M ρₑ ρ ϕ) {[ m₁ ]}).
 
   Definition is_total_function M f (d c : propset (Domain M)) ρₑ ρ :=
     ∀ (m₁ : Domain M),
       m₁ ∈ d ->
       ∃ (m₂ : Domain M),
         m₂ ∈ c /\
-        app_ext (@pattern_interpretation M ρₑ ρ f) {[ m₁ ]}
+        app_ext (@eval M ρₑ ρ f) {[ m₁ ]}
         = {[ m₂ ]}.
 
   Definition total_function_is_injective M f (d : propset (Domain M)) ρₑ ρ :=
@@ -2429,12 +2429,12 @@ Section semantics.
         m₁ = m₂.
 
   Definition is_functional_pattern ϕ M ρₑ ρₛ :=
-    ∃ (m : Domain M), @pattern_interpretation M ρₑ ρₛ ϕ = {[ m ]}.
+    ∃ (m : Domain M), @eval M ρₑ ρₛ ϕ = {[ m ]}.
 
   Lemma functional_pattern_inj ϕ M ρₑ ρ m₁ m₂ :
     @is_functional_pattern ϕ M ρₑ ρ ->
-    m₁ ∈ @pattern_interpretation M ρₑ ρ ϕ ->
-    m₂ ∈ @pattern_interpretation M ρₑ ρ ϕ ->
+    m₁ ∈ @eval M ρₑ ρ ϕ ->
+    m₂ ∈ @eval M ρₑ ρ ϕ ->
     m₁ = m₂.
   Proof.
     intros [m Hm] Hm₁ Hm₂.
